examples/cells: Port to generalized postconditions

src/Rupicola/Examples/Cells/Swap.v
@@ -5,28 +5,33 @@ Section with_parameters.
   Context {semantics : Semantics.parameters}
           {semantics_ok : Semantics.parameters_ok semantics}.
 
-Definition swap_gallina_spec (c1 c2: cell) :=
-  let/d v1 := get c1 in
-  let/d v2 := get c2 in
-  let/d c1 := put v2 c1 in
-  let/d c2 := put v1 c2 in
-  (c1, c2).
+  Definition swap_gallina_spec (c1 c2: cell) :=
+    let/n v1 := get c1 in
+    let/n v2 := get c2 in
+    let/n c1 := put v2 c1 in
+    let/n c2 := put v1 c2 in
+    (c1, c2).
 
-Derive swap_body SuchThat
-       (let swap := ("swap", (["a"; "b"], [], swap_body)) in
-        program_logic_goal_for swap
-        (forall functions,
-         forall a_ptr a b_ptr b tr R mem,
-           sep (TwoCells a_ptr b_ptr (a,b) []) R mem ->
-           WeakestPrecondition.call
-             (swap :: functions)
-             "swap"
-             tr mem [a_ptr;b_ptr]
-             (postcondition_func_norets
-                (TwoCells a_ptr b_ptr (swap_gallina_spec a b))
-                R tr)))
-  As swap_body_correct.
-Proof.
-  compile.
-Qed.
+  Derive swap_body SuchThat
+         (let swap := ("swap", (["c1"; "c2"], [], swap_body)) in
+          program_logic_goal_for swap
+          (forall functions,
+           forall c1_ptr c1 c2_ptr c2 tr R mem,
+             sep (TwoCells c1_ptr c2_ptr (c1, c2) []) R mem ->
+             WeakestPrecondition.call
+               (swap :: functions)
+               "swap"
+               tr mem [c1_ptr; c2_ptr]
+               (postcondition_func_norets
+                  (TwoCells c1_ptr c2_ptr (swap_gallina_spec c1 c2))
+                  R tr)))
+    As swap_body_correct.
+  Proof.
+    compile.
+  Qed.
 End with_parameters.
+
+(* Require Import bedrock2.NotationsCustomEntry. *)
+(* Require Import bedrock2.NotationsInConstr. *)
+(* Arguments swap_body /. *)
+(* Eval simpl in swap_body. *)
