src/Rupicola/Examples/Cells/Cells.v
@@ -1,6 +1,6 @@
 Require Import Rupicola.Lib.Api.
 
-Section with_semantics.
+Section with_parameters.
   Context {semantics : Semantics.parameters}
           {semantics_ok : Semantics.parameters_ok semantics}.
   Record cell := { data : Semantics.word }.
@@ -12,43 +12,39 @@ Section with_semantics.
   Definition OneCell c_ptr c
     : list word -> Semantics.mem -> Prop :=
     fun _ => cell_value c_ptr c.
-  Hint Unfold OneCell : compiler.
 
   Definition TwoCells a_ptr b_ptr ab
     : list word -> Semantics.mem -> Prop :=
     fun _ =>
       sep (cell_value a_ptr (fst ab)) (cell_value b_ptr (snd ab)).
-  Hint Unfold TwoCells : compiler.
 
   Definition get c := c.(data).
   Definition put v (c: cell) := {| data := v |}.
 
   Lemma compile_get :
     forall (locals: Semantics.locals) (mem: Semantics.mem)
-           (locals_ok : Semantics.locals -> Prop)
-           tr retvars R R' functions
-           T (pred: T -> list word -> Semantics.mem -> Prop)
-           c c_ptr c_var k k_impl,
-    forall var,
-      sep (cell_value c_ptr c) R' mem ->
+      tr R functions
+      T (pred: T -> predicate)
+      c c_ptr c_var k k_impl var,
+
+      sep (cell_value c_ptr c) R mem ->
       map.get locals c_var = Some c_ptr ->
+
       let v := (get c) in
-      (let head := v in
-       find k_impl
-       implementing (pred (k head))
-       and-returning retvars
-       and-locals-post locals_ok
-       with-locals (map.put locals var head)
-       and-memory mem and-trace tr and-rest R
-       and-functions functions) ->
-      (let head := v in
-       find (cmd.seq (cmd.set var (expr.load access_size.word (expr.var c_var)))
-                     k_impl)
-       implementing (pred (dlet head k))
-       and-returning retvars
-       and-locals-post locals_ok
-       with-locals locals and-memory mem and-trace tr and-rest R
-       and-functions functions).
+      (let v := v in
+       <{ Trace := tr;
+          Memory := mem;
+          Locals := map.put locals var v;
+          Functions := functions }>
+       k_impl
+       <{ pred (k v) }>) ->
+      <{ Trace := tr;
+         Memory := mem;
+         Locals := locals;
+         Functions := functions }>
+      cmd.seq (cmd.set var (expr.load access_size.word (expr.var c_var)))
+              k_impl
+      <{ pred (nlet [var] v k) }>.
   Proof.
     intros.
     repeat straightline.
@@ -68,55 +64,43 @@ Section with_semantics.
 
   Lemma compile_put :
     forall (locals: Semantics.locals) (mem: Semantics.mem)
-           (locals_ok : Semantics.locals -> Prop)
-           tr retvars R R' functions
-           T (pred: T -> list word -> _ -> Prop)
-           c c_ptr c_var x x_var k k_impl,
-      sep (cell_value c_ptr c) R' mem ->
+      tr R functions
+      T (pred: T -> predicate)
+      c c_ptr c_var x x_var k k_impl,
+      sep (cell_value c_ptr c) R mem ->
       map.get locals c_var = Some c_ptr ->
       map.get locals x_var = Some x ->
       let v := (put x c) in
-      (let head := v in
+      (let v := v in
        forall m,
-         sep (cell_value c_ptr head) R' m ->
-         (find k_impl
-          implementing (pred (k head))
-          and-returning retvars
-          and-locals-post locals_ok
-          with-locals locals
-          and-memory m and-trace tr and-rest R
-          and-functions functions)) ->
-      (let head := v in
-       find (cmd.seq (cmd.store access_size.word (expr.var c_var) (expr.var x_var))
-                     k_impl)
-       implementing (pred (dlet head k))
-       and-returning retvars
-       and-locals-post locals_ok
-       with-locals locals and-memory mem and-trace tr and-rest R
-       and-functions functions).
+         sep (cell_value c_ptr v) R m ->
+         (<{ Trace := tr;
+             Memory := m;
+             Locals := locals;
+             Functions := functions }>
+          k_impl
+          <{ pred (k v) }>)) ->
+      <{ Trace := tr;
+         Memory := mem;
+         Locals := locals;
+         Functions := functions }>
+      cmd.seq (cmd.store access_size.word (expr.var c_var) (expr.var x_var))
+              k_impl
+      <{ pred (nlet [c_var] v k) }>.
   Proof.
     intros.
     unfold cell_value in *.
     repeat straightline.
-    exists c_ptr.
-    split.
-    { repeat straightline; eauto. }
-    { eexists; split.
-      { repeat straightline; eauto. }
-      repeat straightline.
-      subst v; simpl.
-      match goal with
-      | [ H: context[WeakestPrecondition.cmd] |- _ ] => apply H
-      end.
-      eassumption. }
+    exists c_ptr; split; eexists; split; eauto.
+    - repeat straightline; eexists; split; eauto.
+    - repeat straightline; eauto.
   Qed.
-End with_semantics.
+End with_parameters.
+
 Hint Unfold OneCell TwoCells : compiler.
 
 Ltac cell_compile_step :=
-  gen_sym_inc;
-  let name := gen_sym_fetch "v" in
-  first [simple eapply compile_get with (var := name) |
+  first [simple eapply compile_get |
          simple eapply compile_put].
 
 Ltac compile_custom ::=
