src/Rupicola/Examples/Cells/Incr.v
@@ -1,28 +1,27 @@
 Require Import Rupicola.Lib.Api.
 Require Import Rupicola.Examples.Cells.Cells.
-Local Infix "~>" := cell_value.
 
-Section with_semantics.
+Section with_parameters.
   Context {semantics : Semantics.parameters}
           {semantics_ok : Semantics.parameters_ok semantics}.
 
   Definition incr_gallina_spec (c: cell) :=
-    let/d v := get c in
-    let/d one := word.of_Z 1 in
-    let/d v := word.add v one in
-    let/d c := put v c in
+    let/n v := get c in
+    let/n one := word.of_Z 1 in
+    let/n v := word.add v one in
+    let/n c := put v c in
     c.
 
   Instance spec_of_incr : spec_of "incr" :=
     (forall! (c_ptr : address) (c :cell),
-        (sep (c_ptr ~> c))
+        (sep (cell_value c_ptr c))
           ===>
           "incr" @ [c_ptr]
           ===>
           (OneCell c_ptr (incr_gallina_spec c))).
 
-  Derive body SuchThat
-         (let incr := ("incr", (["c_ptr"], [], body)) in
+    Derive body SuchThat
+         (let incr := ("incr", (["c"], [], body)) in
           program_logic_goal_for
             incr
             (ltac:(let x := program_logic_goal_for_function
@@ -30,11 +29,11 @@ Section with_semantics.
                    exact x)))
          As body_correct.
   Proof.
-    cbv [spec_of_incr].
     compile.
   Qed.
+End with_parameters.
 
-  (* Require Import bedrock2.NotationsCustomEntry. *)
-  (* Require Import bedrock2.NotationsInConstr. *)
-  (* Print body. *)
-End with_semantics.
+(* Require Import bedrock2.NotationsCustomEntry. *)
+(* Require Import bedrock2.NotationsInConstr. *)
+(* Arguments body /. *)
+(* Eval simpl in body. *)
